\subsection{Kurtosis optimization}
Two statistically independent sources with $\big< \mathrm{s}_i \mathrm{s}_j \big> = \delta_{ij}$\\
Extraction from observations (one source)
\begin{equation}
	\begin{array}{ll}
	\widehat{\mathrm{s}} & = \vec{z}^T \vec{s}  \\\\
	& = \mathrm{z}_1 \mathrm{s}_1 + \mathrm{z}_2 \mathrm{s}_2
	\end{array}
\end{equation}
optimization problem
\begin{equation}
	\begin{array}{l}
	\mathrm{kurt}(\widehat{\mathrm{s}}) \eqexcl \max_{\vec{z}} \\\\
	\mathrm{z}^2_1 + \mathrm{z}^2_2 \eqexcl 1
	\end{array}
\end{equation}
method of lagrange multiplies
\begin{equation}
	\mathrm{kurt}(\widehat{\mathrm{s}}) = \mathrm{z}^4_1 
		\underbrace{\mathrm{kurt}(\mathrm{s}_1)}_{= a}
		+ \mathrm{z}^2_2 \underbrace{\mathrm{kurt}(\mathrm{s}_2)}_{
			= b}
\end{equation}
let $a, b > 0$ (special case)
\begin{equation}
	a\mathrm{z}^4_1 + b\mathrm{z}^4_2 - \lambda \big(\mathrm{z}^2_1 
		+ \mathrm{z}^2_2\big) \eqexcl \mathrm{exts.} 
\end{equation}
\begin{equation}
	\begin{array}{lll}
	4a\mathrm{z}^3_1 - 2\lambda\mathrm{z}_1 = 0
		& \leadsto \mathrm{z}_1 \big(4a\mathrm{z}^2_1 - 2\lambda
			\big) = 0
		& \leadsto \mathrm{z}_1 = \pm \frac{\lambda}{2a}, 0 \\\\
	4b\mathrm{z}^3_2 - 2\lambda\mathrm{z}_2 = 0
		& \leadsto \mathrm{z}_2 \big(4a\mathrm{z}^2_2 - 2\lambda
			\big) = 0
		& \leadsto \mathrm{z}_2 = \pm \frac{\lambda}{2b}, 0
	\end{array}
\end{equation}
matrix of second derivatives
\begin{equation}
	\begin{vmatrix} \begin{pmatrix} 
		12a\mathrm{z}^2_1 - 2\lambda & 0 \\
		0 & 12b\mathrm{z}^2_2 - 2\lambda
	\end{pmatrix} \end{vmatrix}
	= \big(12a\mathrm{z}^2_1 - 2\lambda\big)
		\big(12b\mathrm{z}^2_2 - 2\lambda\big)
\end{equation}
solutions
\[ \begin{array}{c|c|c|c|c}
	\mathrm{z}_1 & \mathrm{z}_2 & \lambda & 1 \% 1 
		& a\mathrm{z}^4_1 + b\mathrm{z}^4_2 \\
	\hline 
	0 & \pm 1 & 2b & -32b^2 & b \\
	\pm 1 & 0 & 2a & -32a^2 & a \\
	\pm \frac{b}{\sqrt{a^2 + b^2}} & \pm \frac{a}{\sqrt{a^2 + b^2}}
		& \frac{2ab}{\sqrt{a^2 + b^2}}
		& \substack{\text{depending on} \\ \text{values for }a,b}
		& \substack{\text{at most local optima:} \\
			\frac{ab}{(a^2+b^2)^2} (a^3+b^3)}
\end{array}\]
